wip

proof/crefine/RISCV64/SR_lemmas_C.thy
@@ -2224,21 +2224,6 @@ lemma fault_message_length_relationD:
   shows "fault_message_length_relation fmi \<Longrightarrow> length (fmi_reg fmi) = CARD('len)"
   by (simp add: fault_message_length_relation_def)
 
-lemma fault_message_relationE:
-  fixes fmi :: "('struct::mem_type, 'len::finite) fault_message_info"
-  assumes r: "fault_message_relation_unguarded fmi ch"
-  assumes i: "i < CARD('len)"
-  assumes m: "\<And>c_msg. \<lbrakk> ch (fmi_ptr fmi) = Some c_msg;
-                         fmi_msg fmi c_msg.[i] = register_from_H (fmi_reg fmi ! i) \<rbrakk>
-                       \<Longrightarrow> P"
-  shows P
-  using r i fault_message_relation_unguarded_length[OF r]
-  apply (clarsimp simp: fault_message_relation_unguarded_def)
-  apply (erule m)
-  apply (drule arg_cong[where f="\<lambda>xs. xs ! i"])
-  apply (simp add: fault_message_length_relationD list_array_nth)
-  done
-
 lemma syscall_fault_message_length_relation[simp, intro!]:
   "fault_message_length_relation syscall_fault_message_info"
   by (auto simp: syscall_fault_message_info_def fault_message_length_relation_def
@@ -2270,6 +2255,32 @@ lemmas rf_sr_fault_message_relation_unguarded_lemmas
   = rf_sr_exception_fault_message_relation_unguarded
     rf_sr_syscall_fault_message_relation_unguarded
 
+definition fault_message_field_ti ::
+  "('struct::mem_type, 'len::finite) fault_message_info \<Rightarrow> bool"
+  where
+  "fault_message_field_ti fmi
+   \<equiv> field_ti TYPE('struct) [''msg_C'']
+         = Some (adjust_ti (typ_info_t TYPE(machine_word['len])) (fmi_msg fmi) (fmi_upd fmi \<circ> K))
+      \<and> export_uinfo (adjust_ti (typ_info_t TYPE(machine_word['len])) (fmi_msg fmi) (fmi_upd fmi \<circ> K))
+         = export_uinfo (typ_info_t TYPE(machine_word['len]))"
+
+lemma fault_message_field_tiD:
+  fixes fmi :: "('struct::mem_type, 'len::finite) fault_message_info"
+  assumes "fault_message_field_ti fmi"
+  shows "field_ti TYPE('struct) [''msg_C'']
+         = Some (adjust_ti (typ_info_t TYPE(machine_word['len])) (fmi_msg fmi) (fmi_upd fmi \<circ> K))"
+        "export_uinfo (adjust_ti (typ_info_t TYPE(machine_word['len])) (fmi_msg fmi) (fmi_upd fmi \<circ> K))
+         = export_uinfo (typ_info_t TYPE(machine_word['len]))"
+  using assms by (auto simp: fault_message_field_ti_def)
+
+lemma exception_fault_message_field_ti[simp, intro!]:
+  "fault_message_field_ti exception_fault_message_info"
+  by (simp add: fault_message_field_ti_def)
+
+lemma syscall_fault_message_field_ti[simp, intro!]:
+  "fault_message_field_ti syscall_fault_message_info"
+  by (simp add: fault_message_field_ti_def)
+
 lemma fault_message_relation_h_t_valid_global:
   assumes fmi: "fault_message_relation_unguarded fmi (clift hrs)"
   assumes ptr: "p = fmi_ptr fmi"
@@ -2280,13 +2291,26 @@ lemma fault_message_relation_h_t_valid_global:
 lemma fault_message_relation_h_t_valid_array:
   fixes fmi :: "('struct::mem_type, 'len::array_max_count) fault_message_info"
   assumes fmi: "fault_message_relation_unguarded fmi (clift hrs)"
-  assumes ti: "field_ti TYPE('struct) [''msg_C'']
-               = Some (adjust_ti (typ_info_t TYPE(machine_word['len])) (fmi_msg fmi) (fmi_upd fmi \<circ> K))"
-  assumes uinfo: "export_uinfo (adjust_ti (typ_info_t TYPE(machine_word['len])) (fmi_msg fmi) (fmi_upd fmi \<circ> K))
-                  = export_uinfo (typ_info_t TYPE(machine_word['len]))"
+  assumes ti: "fault_message_field_ti fmi"
   shows "hrs_htd hrs \<Turnstile>\<^sub>t PTR(machine_word['len]) &(fmi_ptr fmi\<rightarrow>[''msg_C''])"
   by (rule h_t_valid_field[where 'b="machine_word['len]"
-                           , OF fault_message_relation_h_t_valid_global[OF fmi refl] ti uinfo])
+                           , OF fault_message_relation_h_t_valid_global[OF fmi refl]
+                                fault_message_field_tiD[OF ti]])
+
+lemma fault_message_relationE:
+  fixes fmi :: "('struct::mem_type, 'len::finite) fault_message_info"
+  assumes r: "fault_message_relation_unguarded fmi ch"
+  assumes i: "i < CARD('len)"
+  assumes m: "\<And>c_msg. \<lbrakk> ch (fmi_ptr fmi) = Some c_msg;
+                         fmi_msg fmi c_msg.[i] = register_from_H (fmi_reg fmi ! i) \<rbrakk>
+                       \<Longrightarrow> P"
+  shows P
+  using r i fault_message_relation_unguarded_length[OF r]
+  apply (clarsimp simp: fault_message_relation_unguarded_def)
+  apply (erule m)
+  apply (drule arg_cong[where f="\<lambda>xs. xs ! i"])
+  apply (simp add: fault_message_length_relationD list_array_nth)
+  done
 
 end
 end
